Tighten cost bounds for `listOf` + Add combinators/proofs for non-empty lists / strings (#11)
* Add combinator for non-empty lists/strings + monotonicity proof

* support_nonEmptyListOf

* add simp lemma

* Add some tests

* Add cost lemma IsBounded_nonEmptyListOf

* Use a slightly tighter cost function bound

* Add termination proof for nonEmptyListOf

* NonEmptyString.arbitrary_support

* NonEmptyString.arbitrary_terminates

* Tighten cost bounds for listOf / nonEmptyListOf

* Get rid of genCharList, rewrite String.arbitrary in terms of listOf, tighten cost-bounds for string generators

* Fix compilation errors

Basalt/Combinators.lean
@@ -133,6 +133,21 @@ def listOf [Gen G] (g : G α) : G (List α) := do
       return x :: xs)
 partial_fixpoint
 
+/-- Generates a *non-empty* list with unbounded length,
+    where each element is produced using `g`. -/
+def nonEmptyListOf {G α} [Gen G] (g : G α) : G (List α) := do
+  -- Ideally, one would write the first sub-generator as `fun _ => List.singleton <$> g`,
+  -- but there are no monotonicity lemmas for `<$>` in `Lean.Order` and
+  -- rewriting `<$>` in terms of `bind` requires a `LawfulMonad` instance (but `G` is only a `Monad`),
+  -- so we have to express it using an explicit `bind`
+  RandomChoice.pick
+    (fun () => do let x ← g; pure [x])
+    (fun () => do
+      let x ← g
+      let xs ← nonEmptyListOf g
+      return x :: xs)
+partial_fixpoint
+
 /-- Define a partial order over `List α` that says `l1 ⊑ l2` when:
 - `l1.length = l2.length`
 - `l1[i] ⊑ l2[i]` for all list elements (here we are comparing them using the `PartialOrder` on `α`) -/
@@ -551,6 +566,50 @@ theorem monotone_listOf [Gen G] {γ : Sort w} [PartialOrder γ]
     split
     · -- Non-recursive branch: both sides return the empty list
       apply PartialOrder.rel_refl
+    · -- Recursive branch: `bind (g x) … ⊑ bind (g y) …`
+      apply PartialOrder.rel_trans (MonoBind.bind_mono_left (hg x y hxy))
+      apply MonoBind.bind_mono_right
+      intro a
+      apply MonoBind.bind_mono_left
+      assumption
+
+
+/-- Lemma allowing us to use `nonEmptyListOf` in functions marked as `partial_fixpoint`
+    (the `monotonicity` tactic is used under the hood by `partial_fixpoint`).
+
+    Note: the body of this proof is very similar to `monotone_listOf`. -/
+@[partial_fixpoint_monotone]
+theorem monotone_nonEmptyListOf [Gen G] {γ : Sort w} [PartialOrder γ]
+    (g : γ → G α) (hg : monotone g) :
+    monotone (fun x => nonEmptyListOf (g x)) := by
+  unfold monotone
+  intro x y hxy
+  show nonEmptyListOf (g x) ⊑ nonEmptyListOf (g y)
+  -- Convert the RHS to a variable `z` so that we only delta-reduce `nonEmptyListOf` on the LHS
+  generalize hw : nonEmptyListOf (g y) = w
+  delta nonEmptyListOf
+  apply Lean.Order.fix_induct (motive := fun z => z ⊑ w)
+  · -- Admissibility: a chain's supremum is ⊑ `w`
+    -- iff every chain element is ⊑ `w`
+    intro c hc hall
+    apply Lean.Order.csup_le <;> assumption
+  · -- Induction step: assuming `z ⊑ w` (where `w = listOf (g y)`),
+    -- one unfolding of `nonEmptylistOf`'s body is still ⊑ `w`.
+    intro z hz
+    subst hw
+    unfold nonEmptyListOf
+    -- Both sides of the ⊑ are now in terms of `pick` only
+    simp only [RandomChoice.pick]
+    -- Both sides now in terms of `bind` and `choose` only
+    apply MonoBind.bind_mono_right
+    intro n
+    -- Case on which branch `pick` selects
+    split
+    · -- Non-recursive branch: both sides return a singleton list
+      unfold monotone at hg
+      apply MonoBind.bind_mono_left
+      apply hg
+      assumption
     · -- Recursive branch: `bind (g x) … ⊑ bind (g y) …`
       apply PartialOrder.rel_trans (MonoBind.bind_mono_left (hg x y hxy))
       apply MonoBind.bind_mono_right
