BasaltExamples/ArbString/Def.lean
@@ -4,6 +4,7 @@ Released under MIT license as described in the file LICENSE.
 Authors: Harrison Goldstein
 -/
 import Basalt.Gen
+import Basalt.Combinators
 import BasaltExamples.ArbChar.Def
 
 open RandomChoice ArbChar
@@ -19,18 +20,12 @@ recursive generator of alphanumeric character lists with the same subcritical sh
 
 namespace ArbString
 
-/-- Helper function: generates a random list of alphanumeric characters -/
-def genCharList [Gen G] : G (List Char) :=
-  pick
-    (fun _ => pure [])
-    (fun () => do
-      let x ← Char.arbitrary
-      let xs ← genCharList
-      return x :: xs)
-partial_fixpoint
-
-/-- Generates a random alphanumeric string -/
+/-- Generates a random (possibly empty) alphanumeric string -/
 def String.arbitrary [Gen G] : G String :=
-  String.ofList <$> genCharList
+  String.ofList <$> listOf Char.arbitrary
+
+/-- Generates a random, non-empty alphanumeric string -/
+def NonEmptyString.arbitrary [Gen G] : G String :=
+  String.ofList <$> nonEmptyListOf Char.arbitrary
 
 end ArbString
