BasaltTest/PlausibleGen.lean
@@ -1,12 +1,27 @@
 import BasaltExamples.BST
 import BasaltExamples.Heap
+import BasaltExamples.ArbString
+import BasaltExamples.ArbNat
 
 /- `genBST` can be run in `PlausibleGen`. -/
 #guard_msgs(drop info) in
 #eval (for _ in [0:20] do
   IO.println <| repr (← Plausible.Gen.run (BST.Tree.genBST (G := Plausible.Gen) 0 10) 10) : IO Unit)
 
-/- `genHeap` can be run in `PlausibleGen`. -/
+/- `genHeap` can be run in `PlausibleGen`.
+    Note: on Lean 4.29 (where the Lean interpreter's default stack size is smaller compared to Lean 4.33),
+    trying to run this generator with `fuel = 10` causes stack overflow, so on Lean 4.29,
+    we lower the fuel to 3. -/
 #guard_msgs(drop info) in
-#eval (for _ in [0:20] do
-  IO.println <| repr (← Plausible.Gen.run (Heap.Tree.genHeap (G := Plausible.Gen) 0) 10) : IO Unit)
+#eval (for _ in [0:10] do
+  IO.println <| repr (← Plausible.Gen.run (Heap.Tree.genHeap (G := Plausible.Gen) 0) 3) : IO Unit)
+
+/- `NonEmptyString.arbitrary` can be run in `PlausibleGen`. -/
+#guard_msgs(drop info) in
+#eval (for _ in [0:5] do
+  IO.println <| repr (← Plausible.Gen.run (ArbString.NonEmptyString.arbitrary (G := Plausible.Gen)) 10) : IO Unit)
+
+/- `nonEmptyListOf Nat.arbirary` can be run in `PlausibleGen`.  -/
+#guard_msgs(drop info) in
+#eval (for _ in [0:5] do
+  IO.println <| repr (← Plausible.Gen.run (nonEmptyListOf ArbNat.Nat.arbitrary (G := Plausible.Gen)) 10) : IO Unit)
